proof/crefine/ARM_HYP/Detype_C.thy
@@ -1833,14 +1833,13 @@ proof -
   }
   moreover
   {
-    assume "s' \<Turnstile>\<^sub>c (Ptr::(32 word \<Rightarrow> (pde_C[2048]) ptr)) (symbol_table ''armUSGlobalPD'')"
+    assume "s' \<Turnstile>\<^sub>c armUSGlobalPD_Ptr"
     moreover
-    from sr ptr_refs have "ptr_span (pd_Ptr (symbol_table ''armUSGlobalPD''))
+    from sr ptr_refs have "ptr_span armUSGlobalPD_Ptr
       \<inter> {ptr..ptr + 2 ^ bits - 1} = {}"
       by (fastforce simp: rf_sr_def cstate_relation_def Let_def)
     ultimately
-    have "hrs_htd (hrs_htd_update (typ_region_bytes ptr bits) (t_hrs_' (globals s')))
-      \<Turnstile>\<^sub>t (Ptr::(32 word \<Rightarrow> (pde_C[2048]) ptr)) (symbol_table ''armUSGlobalPD'')"
+    have "hrs_htd (hrs_htd_update (typ_region_bytes ptr bits) (t_hrs_' (globals s'))) \<Turnstile>\<^sub>t armUSGlobalPD_Ptr"
       using al wb
       apply (cases "t_hrs_' (globals s')")
       apply (simp add: hrs_htd_update_def hrs_htd_def h_t_valid_typ_region_bytes upto_intvl_eq)
